% Titre : somme
% Filiere : BCPST
% Difficulte : 
% Type : TD 
% Categories :somme
% Subcategories : 
% Keywords : somme




\begin{exercice}  \;
\noindent Soit $n\in\N,\ n\geq 3$. Simplifier les nombres suivants:
$$A=\ddp\frac{7!}{6!},\ \ \ \ B=\ddp\frac{3\times 4!}{(3!)^2},\ \ \ \ 
C=\ddp\frac{n!}{(n-1)!},\ \ \ \ D=\ddp\frac{(n+1)!}{(n-3)!}\ \ \hbox{et}\ \ E=\ddp\frac{(n+1)!}{(n-2)!}+\ddp\frac{n!}{(n-1)!}.$$
\end{exercice}


\%\%\%\%\%\%\%\%\%\%\%\%\%\%\%\%\%\%\%\%
\%\%\%\%\%\%\%\%\%\%\%\%\%\%\%\%\%\%\%\%
\%\%\%\%\%\%\%\%\%\%\%\%\%\%\%\%\%\%\%\%




\begin{correction}  \; \vsec
\begin{itemize}
\item[$\bullet$] $A=\ddp\frac{7!}{6!}=\ddp\frac{7\times 6!}{6!}=\fbox{$7.$}$
\item[$\bullet$] $B=\ddp\frac{3\times 4!}{(3!)^2}=\ddp\frac{3\times 4\times 3!}{3!\times 3\times 2}=\fbox{$2$.}$
\item[$\bullet$] $C=\ddp\frac{n!}{(n-1)!}=\ddp\frac{n\times (n-1)!}{(n-1)!}=\fbox{$n$.}$
\item[$\bullet$] $D=\ddp\frac{(n+1)!}{(n-3)!}=\ddp\frac{(n+1)\times n\times (n-1)\times (n-2)\times (n-3)!}{(n-3)!}=\fbox{$(n+1) n (n-1) (n-2)$.}$
\item[$\bullet$] $E=\ddp\frac{(n+1)!}{(n-2)!}+\ddp\frac{n!}{(n-1)!}=(n+1)n(n-1)+n=n(n^2-1+1)=\fbox{$n^3$.}$
\end{itemize}
\end{correction}